# The Noether and Artin Properties for Rings and Modules

??? definition "Definition: Module"
    A module $M$ over $R$ is a vector space over $R$.


??? remark
    === "Basis"
        Not every module has a basis.
    === "Free modules"
        A module with a basis is called free.
    === "Free vector spaces"
        All vector spaces (modules over fields) are free.


??? example
    $\Z/(2)$ is a $\Z$-module:

    $a (b + (2)) = ab + (2)$


??? notation
    $m_1, ..., m_n \in M$
    
    $(m_1, ..., m_n)_R = (m_1, ..., m_n)$ is the submodule generated by $m_1, ..., m_n$, which
    consists of all $R$-linear combinations.


??? definition "Definition 2.1"
    ## Noetherian and artinian rings and modules
    Let $R$ be a ring and $M$ be a module.

    Ascending chain condition = a.c.c </br>
    Descending chain condition = (d.c.c)

    === "Noetherian module"
        $M$'s submodules satisfies a.c.c.
    === "Noetherian ring"
        $R$'s ideals satisfy a.c.c
    === "Artinian module"
        $M$'s submodules satisfies d.c.c.
    === "Artinian ring"
        $R$'s ideals satisfies d.c.c.


??? example "Example 2.2"
    === "$R=\Z$"
        $I_n \ideal \Z \iff I_n = (a_n)$ for some $a_n \in \Z$

        Assume $\{I_n\}$ is an acsending chain.

        $\implies a_{n+1} | a_n$.

        This has to stop.

        $\implies \Z$ is artinean

    === "$K[x]$"
        $K[x]$ is noetheriam by the same arguments as for $R=\Z$

    === "$R=K^S$"
        Let $S$ be an infinite set

        $R = K^S = \{f : S \to K\}$ with pointwise addition and multiplication.

        $Y \subseteq S$ any subset

        $I_Y:=\{f \in R : f(Y) = \{0\}\}$ is an ideal.

        $Y_1 \subsetneq Y_2 \implies I_{Y_1} \supsetneq I_{Y_2}$

        Then there exists an infinite strictly descending chain of strict subsets, thus an
        infinite strict ascending chain of ideals.

        $\implies R$ is not Noetherian.

    === "$\Z$ or $K[x]$"
        Neither $\Z$ nor $K[x]$ are Artinian. Consider $I_i = (2^i)$

    === "Fields and finite rings"
        are both Artinian and Noetherian.

??? example "Example 2.3"
    $K[x, xy, xy^2, ...] \subseteq K[x, y]$ is not Noetherian.


??? proposition "Proposition 2.4"
    ## Submodules and quotient modules <a id=l24></a>

    Let $M$ be an $R$-module, and $N\subseteq M$ be a sumbodule.

    === "Proposition"
        $$
        M \text{ is Noetherian/Artinian } \iff N \land M/N \text{ is Noetherian/Artinian}
        $$
    === "Proof"
        The proof for artinian follows from tha same arguments.

        === "$\implies$"

            $M$ is Noetherian $\implies N$ is Noetherian.
    
            Let $U_1 \subseteq U_2 \subseteq ... \subseteq M/N$ be a chain, and 
    
            $$
            \begin{align*}
                \phi : M & \to M/N \\
                m & \mapsto m + N
            \end{align*}
            $$
    
            be a homomorphism.
    
            $$
            \begin{align*}
                \implies & \phi^{-1}(U_1) \subseteq \phi^{-1}(U_2) \subseteq ...   \subseteq M \text{ stabilizes} \\
                \implies & U_1 \subseteq U_2  \subseteq ... \subseteq M/N \text{ must stabilize.}
            \end{align*}
            $$

        === "$\impliedby$"
            Let $M_1 \subseteq M_2 \subseteq ... \subseteq M$ be a chain.
    
            $$
            \begin{align*}
                \implies &
                \begin{cases}
                    \phi(M_1) & \subseteq \phi(M_2) & \subseteq ... & \subseteq M/N \\
                    N \cap M_1 & \subseteq N \cap M_2 & \subseteq ... & \subseteq N
                \end{cases} \\
                \implies &\exists\ n\in\N \text{ s.t.} \\
                & \begin{rcases}
                    \phi(M_i) = \phi(M_n) \\
                    N \cap M_i = N \cap M_n
                \end{rcases} \ \forall i > n
            \end{align*}
            $$
    
            We claim that $M_i = M_n \ \forall\ i>n$:
    
            Let $m \in M_i$.
        
            $$
            \begin{align*}
                \implies & \phi(m) \in \phi(M_i) = \phi(M_n) \\
                \implies & \exists\ m' \in M_n \text{ s.t.} \\
                & m'-m \in N \cap M_i = N \cap M_n \\
                \implies & m = (m - m') + m1 \in M_n & \square
            \end{align*}
            $$


??? definition "Definition 2.5"
    ## Ideal Product
    
    $\begin{align*}
        \text{Let } & I \ideal R \\
        & M \text{ be an } R \text{-module}
    \end{align*}$

    === "Product"
        $$I \cdot M = \left\{\sum_{i=1}^n a_i m_i | n\in\N, a_i\in I, m_i\in\ M\right\} \subseteq M$$

    === "Ideal Product"
        $M = J \ideal R$

        $$M \cdot I \ideal R$$

        This is commutative and associative.

        $I \cdot J \subseteq I \cap J$

        $\sqrt{I\cdot J} = \sqrt{I \cap J}$

    === "Ideal power"
        $$I^n\\ I^0:=R$$


??? lemma "Lemma 2.6"
    ## Ideal powers and radical ideals

    $\begin{align*}
        \text{Let } & I, J \ideal R \\
        & I \text{ f.g.}
    \end{align*}$

    === "Lemma"
        $$ I \subseteq \sqrt J \iff \exists\ k \in \N : I^k \subseteq J$$

    === "Proof"
        === "$\impliedby$"
            $\begin{align*}
                \text{We have that } & I^k \subseteq J \\
                & a \in I \\
                \implies & a^k \in I^k \subseteq J \\
                \implies & a \in \sqrt J & \square
            \end{align*}$

        === "$\implies$"
            $\begin{align*}
                \text{We have that } & I = (a_1, a_2, ..., a_n) \\
                & I \subseteq \sqrt J \\
                \implies &
                \begin{cases}
                    \exists\ m>0 \text{ s.t.} \\
                    a^m \in J
                \end{cases}
            \end{align*}$

            Let $k:=n(m-1)+1$

            Claim: Every product of k elements from I lies in J. This would imply $I^k \subseteq J$.

            $\begin{align*}
                \text{Let } & x_1, ..., x_k \in I \\
                & x_i = \sum_{j=1}^n r_{ij} a_j & r_{ij}\in R \\
            \end{align*}$

            $\implies \prod_{i=1}^k x_i \in J$, as at least one $a_j$ is picked $m$ times $\tab\square$


??? lemma "Lemma 2.7"
    ## Lemma 2.7 <a id="l27"></a>
    $\begin{align*}
        \text{Let } & m_1, ..., m_n \in \Specmax R \text{ s.t.} \\
        & m_1 \cdot m_2 \cdot ... \cdot m_n = \{0\}
    \end{align*}$

    === "Lemma"
        $$R \text{ is Noetherian } \iff R \text{ is Artinian}$$

        Moreover,

        $$\Spec R = \{m_i\}_1^n$$

    === "Proof"
        Set $I_i = \prod_{j=1}^i m_j \ideal R$

        $\implies \{0\} = I_n \subseteq I_{n-1} \subseteq ... \subseteq I_1 \subseteq I_0 = R$

        By [L.2.4](#l24), we get that

        $$
        R \text{ is }
        \begin{matrix} \text{Noetherian} \\ \text{Artinian} \end{matrix}
        \iff
        I_{i-1}/I_i \text{ is }
        \begin{matrix} \text{Noetherian} \\ \text{Artinian} \end{matrix}\ \ \forall\ i
        $$

        We have that $m_i (I_{i-1}/I_i) = \{0\}$

        $\implies I_{i-1}/I_i$ is a vectorspace over $K_i:=R/m_i$.

        So $I_{i-1}$ is Artinian/Noetherian $\iff \dim_{k_i}(I_{i-1}/I_i) < \infty \tab\square$


???+ theorem "Theorem 2.8"
    ## Artinian rings are Noetherian
    === "Theorem"
        $$R \text{ is Artinian } \iff R \text{ is Noetherian and } \Spec R = \Specmax R$$

    === "Proof"
        === "$\implies$"
            Assume $|\Specmax R|=\infty$
            
            $\implies \ \exists \left\{m_i\right\}_{i\in\N} \subseteq \Specmax R$ which are pairwise distinct.

            Setting
            $\begin{align*}
                I_i = \bigcap_{j=1}^i m_j
            \end{align*}$ yields a decreasing chain.

            $$
            \begin{align*}
                \implies & \exists\ n : I_{n+1} = I_n \\
                \implies & \bigcap_{j=1}^n m_j \subseteq m_{n+1} \\
                \implies &
                \begin{cases}
                    \exists\ j \le n \text{ s.t.} \\
                    m_j \subseteq m_{n+1}
                \end{cases} \implies m_j = m_{n+1} \contradiction\\
                \implies & \Specmax R = \{m_i\}1^k, \text{ for some finite } k \\
            \end{align*}
            $$

            Let 
            $\begin{align*}
                I = \bigcap_{j=1}^k m_j
            \end{align*}$
            
            $$
            \begin{align*}
                \implies & I^i \text{ forms a descending sequence.} \\
                \implies &
                \begin{cases}
                    \exists\ n\in\N \text{ s.t.} \\
                    I^i = I^n =: J \tab\forall i \ge n
                \end{cases} \tab (*)
            \end{align*}
            $$

            If $J = \{0\}$, it follows from [L.2.7](#l27) that $R$ is Artinian. Assume it is not.

            Let $\M := \{J' \ideal R | J' \cdot J \neq \{0\}\} \neq \emptyset$. </br>
            As $R$ is Artinian, $\M$ must have a minimal element $\hat J \in \M$.

            Pick any $x \in \hat J$ s.t. $x J \neq \{0\}$.

            $\implies J \supseteq (x) \in \M$ is a submodule

            $\implies \hat J = (x)$, as $J$ is minimal in $\M$

            From $(*)$, we get

            $$
            \begin{align*}
                & J^2 = I^{2n} = J \\
                & \implies \hat JJ \cdot J = \hat JJ^2 = \hat JJ \neq \{0\} \\
                & \implies \hat J\cdot J \in \M \\
                & \implies \hat J\cdot J = \hat J, \text{ as J is minimal}
            \end{align*}
            $$

            As $\hat J = (x)$ is pricipal, we get

            $$
            \begin{align*}
                & (x) J = (x) \\
                & \implies
                \begin{cases}
                    \exists\ y \in J \text{ s.t.} \\
                    x = xy
                \end{cases}
            \end{align*}
            $$

            As $J \subseteq I \subseteq m_j \ \forall\ j$:

            $$
            \begin{align*}
                \implies& y \in m_j \ \forall\ j \\
                \implies &y-1 \text{ lies in no maximal ideal} \\
                \implies &(y-1) = R \tab\text{generates R}\\
                \implies &y-1 \in R^\times \\
                (y-1)x=0 \implies & x = 0 \contradiction \\
                \implies & J = \{0\} & \square
            \end{align*}
            $$
        
        === "$\impliedby$"
            Postponed